Remove Mathlib from the core computation

Regex/NFA/Basic.lean
@@ -1,5 +1,3 @@
-import Mathlib.Data.Set.Basic
-
 namespace NFA
 
 inductive Node where
@@ -10,59 +8,44 @@ inductive Node where
   | split (next₁ next₂ : Nat)
 deriving Repr
 
-def Node.charStep (n : Node) (c : Char) : Set Nat :=
-  match n with
-  | Node.char c' next => if c == c' then {next} else ∅
-  | _ => ∅
-
-def Node.εStep (n : Node) : Set Nat :=
-  match n with
-  | Node.epsilon next => {next}
-  | Node.split next₁ next₂ => {next₁, next₂}
-  | _ => ∅
-
-def Node.inBounds (n : Node) (size : Nat) : Prop :=
-  (∀ c, n.charStep c ⊆ { j | j < size }) ∧ n.εStep ⊆ { j | j < size }
+def Node.inBounds (node : Node) (size : Nat) : Bool :=
+  match node with
+  | Node.done => true
+  | Node.fail => true
+  | Node.epsilon next => next < size
+  | Node.char _ next => next < size
+  | Node.split next₁ next₂ => next₁ < size && next₂ < size
 
 @[simp]
 theorem Node.inBounds.done {size : Nat} : Node.done.inBounds size := by
-  simp [inBounds, charStep, εStep]
+  simp [inBounds]
 
 @[simp]
 theorem Node.inBounds.fail {size : Nat} : Node.fail.inBounds size := by
-  simp [inBounds, charStep, εStep]
+  simp [inBounds]
 
 @[simp]
 theorem Node.inBounds.epsilon {size next : Nat} (h : next < size) :
   (Node.epsilon next).inBounds size := by
-  simp [inBounds, charStep, εStep, h]
+  simp [inBounds, h]
 
 @[simp]
 theorem Node.inBounds.char {size next : Nat} {c : Char} (h : next < size) :
   (Node.char c next).inBounds size := by
-  simp [inBounds, charStep, εStep]
-  intro c'
-  split <;> simp [h]
+  simp [inBounds, h]
 
 @[simp]
 theorem Node.inBounds.split {size next₁ next₂ : Nat} (h₁ : next₁ < size) (h₂ : next₂ < size) :
   (Node.split next₁ next₂).inBounds size := by
-  simp [inBounds, charStep, εStep]
-  apply Set.insert_subset <;> simp [h₁, h₂]
+  simp [inBounds, h₁, h₂]
 
 theorem Node.inBounds_of_inBounds_of_le {n : Node} (h : n.inBounds size) (le : size ≤ size') :
   n.inBounds size' := by
   simp [inBounds] at *
-  apply And.intro
-  . intro c
-    apply le_trans (h.left c)
-    simp
-    intro j h
-    exact Nat.lt_of_lt_of_le h le
-  . apply le_trans h.right
-    simp
-    intro j h
-    exact Nat.lt_of_lt_of_le h le
+  split <;> simp at h <;> try simp
+  next => exact Nat.lt_of_lt_of_le h le
+  next => exact Nat.lt_of_lt_of_le h le
+  next => exact ⟨Nat.lt_of_lt_of_le h.left le, Nat.lt_of_lt_of_le h.right le⟩
 
 /--
   The NFA consists an array of nodes and a designated start node.
