Regex/NFA/Compile.lean
@@ -1,34 +1,29 @@
 import Regex.Lemmas
 import Regex.Regex
 import Regex.NFA.Basic
-import Regex.NFA.Order
+
+import Std.Data.Array.Lemmas
 
 namespace NFA
 
 def NFA.addNode (nfa : NFA) (node : Node) :
-  { nfa' : NFA // nfa ≤ nfa' } :=
+  { nfa' : NFA // nfa.nodes.size ≤ nfa'.nodes.size } :=
   have isLt : nfa.nodes.size < (nfa.nodes.push node).size := by
     simp [Array.size_push]
   let start := nfa.nodes.size
   let nfa' : NFA := ⟨nfa.nodes.push node, ⟨start, isLt⟩⟩
 
-  have property : nfa ≤ nfa' := by
-    intro i h
-    have h' : i < nfa'.nodes.size := Nat.lt_trans h isLt
-    have eq : nfa'[i] = nfa[i] := by
-      apply Array.get_push_lt
-    exact ⟨h', Node.le_of_eq eq.symm⟩
+  have property : nfa.nodes.size ≤ nfa'.nodes.size := by
+    simp
+    exact Nat.le_succ _
 
   ⟨nfa', property⟩
-
-theorem NFA.le_addNode {nfa : NFA} {node : Node} :
-  nfa ≤ (nfa.addNode node).val := (nfa.addNode node).property
 
 theorem NFA.lt_size_addNode {nfa : NFA} {node : Node} :
   nfa.nodes.size < (nfa.addNode node).val.nodes.size := (nfa.addNode node).val.start.isLt
 
 theorem NFA.get_lt_addNode {nfa : NFA} {node : Node} (h : i < nfa.nodes.size) :
-  (nfa.addNode node).val[i]'(Nat.lt_of_lt_of_le h (NFA.le_size_of_le NFA.le_addNode)) = nfa[i] :=
+  (nfa.addNode node).val[i]'(Nat.lt_trans h lt_size_addNode) = nfa[i] :=
   Array.get_push_lt _ _ _ h
 
 @[simp]
@@ -50,7 +45,7 @@ theorem NFA.get_addNode' {nfa : NFA} {node : Node} :
     simp [NFA.addNode]
   simp [this]
 
-theorem NFA.start_addNode {nfa : NFA} {node : Node} {result : { nfa' : NFA // nfa ≤ nfa' }}
+theorem NFA.start_addNode {nfa : NFA} {node : Node} {result : { nfa' : NFA // nfa.nodes.size ≤ nfa'.nodes.size }}
   (eq : nfa.addNode node = result) :
   result.val.start.val = nfa.nodes.size := by
   rw [←eq]
@@ -69,7 +64,7 @@ where
     Returned NFA contains the compiled nodes at the end and starts at the node
     corresponding to the given regex.
   -/
-  loop (r : Regex) (next : Nat) (nfa : NFA) : { nfa' // nfa ≤ nfa' } := match r with
+  loop (r : Regex) (next : Nat) (nfa : NFA) : { nfa' // nfa.nodes.size ≤ nfa'.nodes.size } := match r with
   | .empty => nfa.addNode .fail
   | .epsilon => nfa.addNode (.epsilon next)
   | .char c => nfa.addNode (.char c next)
@@ -81,21 +76,28 @@ where
     let start₂ := nfa₂.val.start
     let nfa' := nfa₂.val.addNode (.split start₁ start₂)
 
-    have property : nfa ≤ nfa' :=
-      calc nfa
-        _ ≤ nfa₁.val := nfa₁.property
-        _ ≤ nfa₂.val := nfa₂.property
-        _ ≤ nfa' := nfa'.property
+    have property : nfa.nodes.size ≤ nfa'.val.nodes.size :=
+      -- calc nfa
+      --   _ ≤ nfa₁.val := nfa₁.property
+      --   _ ≤ nfa₂.val := nfa₂.property
+      --   _ ≤ nfa' := nfa'.property
+      calc nfa.nodes.size
+        _ ≤ nfa₁.val.nodes.size := nfa₁.property
+        _ ≤ nfa₂.val.nodes.size := nfa₂.property
+        _ ≤ nfa'.val.nodes.size := nfa'.property
 
     ⟨nfa', property⟩
   | .concat r₁ r₂ =>
     let nfa₂ := loop r₂ next nfa
     let nfa₁ := loop r₁ nfa₂.val.start nfa₂
 
-    have property : nfa ≤ nfa₁ :=
-      calc nfa
-        _ ≤ nfa₂.val := nfa₂.property
-        _ ≤ nfa₁.val := nfa₁.property
+    have property : nfa.nodes.size ≤ nfa₁.val.nodes.size :=
+      -- calc nfa
+      --   _ ≤ nfa₂.val := nfa₂.property
+      --   _ ≤ nfa₁.val := nfa₁.property
+      calc nfa.nodes.size
+        _ ≤ nfa₂.val.nodes.size := nfa₂.property
+        _ ≤ nfa₁.val.nodes.size := nfa₁.property
 
     ⟨nfa₁, property⟩
   | .star r =>
@@ -108,693 +110,40 @@ where
     let start := nfa'.val.start
     let nfa'' := loop r start nfa'
 
-    have property : nfa ≤ nfa'' :=
-      calc nfa
-        _ ≤ nfa'.val := nfa'.property
-        _ ≤ nfa''.val := nfa''.property
+    have property : nfa.nodes.size ≤ nfa''.val.nodes.size :=
+      -- calc nfa
+      --   _ ≤ nfa'.val := nfa'.property
+      --   _ ≤ nfa''.val := nfa''.property
+      calc nfa.nodes.size
+        _ ≤ nfa'.val.nodes.size := nfa'.property
+        _ ≤ nfa''.val.nodes.size := nfa''.property
     have isLt : start.val < nfa''.val.nodes.size :=
-      Nat.lt_of_lt_of_le nfa'.val.start.isLt (NFA.le_size_of_le nfa''.property)
+      Nat.lt_of_lt_of_le nfa'.val.start.isLt nfa''.property
 
     -- Patch the placeholder node
     let target := nfa''.val.start
     let nodes''' := nfa''.val.nodes.set ⟨start.val, isLt⟩ (.split target next)
 
+    -- TODO: maybe I should have used Fin.cast
     have eq_size : nodes'''.size = nfa''.val.nodes.size := by simp
     have isLt' : start.val < nodes'''.size := eq_size ▸ isLt
     let nfa''' := ⟨nodes''', ⟨start.val, isLt'⟩⟩
 
-    have property' : nfa ≤ nfa''' := by
-      intro i h
+    have property' : nfa.nodes.size ≤ nfa'''.nodes.size := by
+      simp
+      exact property
+      -- intro i h
 
-      have le_size : nfa.nodes.size ≤ nfa''.val.nodes.size := NFA.le_size_of_le property
-      have h₂ : i < nodes'''.size := Nat.lt_of_lt_of_le h (eq_size ▸ le_size)
-      exists h₂
+      -- have le_size : nfa.nodes.size ≤ nfa''.val.nodes.size := NFA.le_size_of_le property
+      -- have h₂ : i < nodes'''.size := Nat.lt_of_lt_of_le h (eq_size ▸ property)
+      -- exists h₂
 
-      have eq : nfa'''[i] = nfa''.val[i]'(Nat.lt_of_lt_of_le h le_size) := by
-        apply Array.get_set_ne
-        exact (Nat.ne_of_gt h)
-      rw [eq]
-      exact (property i _).2
+      -- have eq : nfa'''[i] = nfa''.val[i]'(Nat.lt_of_lt_of_le h le_size) := by
+      --   apply Array.get_set_ne
+      --   exact (Nat.ne_of_gt h)
+      -- rw [eq]
+      -- exact (property i _).2
 
     ⟨nfa''', property'⟩
-
--- Useful lemmas about the compilation
-theorem compile.loop.le : nfa ≤ (compile.loop r next nfa).val :=
-  (compile.loop r next nfa).property
-
-theorem compile.loop.empty (eq : compile.loop .empty next nfa = result)
-  {motive : result = nfa.addNode .fail → P} : P := by
-  simp [compile.loop] at eq
-  exact motive eq.symm
-
-theorem compile.loop.epsilon (eq : compile.loop .epsilon next nfa = result)
-  {motive : result = nfa.addNode (.epsilon next) → P} : P := by
-  simp [compile.loop] at eq
-  exact motive eq.symm
-
-theorem compile.loop.char (eq : compile.loop (.char c) next nfa = result)
-  {motive : result = nfa.addNode (.char c next) → P} : P := by
-  simp [compile.loop] at eq
-  exact motive eq.symm
-
-theorem compile.loop.alternate (eq : compile.loop (Regex.alternate r₁ r₂) next nfa = result)
-  {motive : ∀nfa₁ start₁ nfa₂ start₂ nfa' property,
-    nfa₁ = compile.loop r₁ next nfa →
-    start₁ = nfa₁.val.start →
-    nfa₂ = compile.loop r₂ next nfa₁ →
-    start₂ = nfa₂.val.start →
-    nfa' = nfa₂.val.addNode (.split start₁ start₂) →
-    result = ⟨nfa', property⟩ →
-    P
-  } : P := by
-  let nfa₁ := loop r₁ next nfa
-  let start₁ := nfa₁.val.start
-  let nfa₂ := loop r₂ next nfa₁
-  let start₂ := nfa₂.val.start
-  let nfa' := nfa₂.val.addNode (.split start₁ start₂)
-
-  have property : nfa ≤ nfa' :=
-    calc nfa
-      _ ≤ nfa₁.val := nfa₁.property
-      _ ≤ nfa₂.val := nfa₂.property
-      _ ≤ nfa' := nfa'.property
-
-  have : result = ⟨nfa', property⟩ := by
-    simp [eq.symm, compile.loop]
-  exact motive nfa₁ start₁ nfa₂ start₂ nfa' property rfl rfl rfl rfl rfl this
-
-theorem compile.loop.concat (eq : compile.loop (Regex.concat r₁ r₂) next nfa = result)
-  {motive : ∀nfa₂ nfa₁ property,
-    nfa₂ = compile.loop r₂ next nfa →
-    nfa₁ = compile.loop r₁ nfa₂.val.start nfa₂ →
-    result = ⟨nfa₁, property⟩ →
-    P
-  } : P := by
-  let nfa₂ := loop r₂ next nfa
-  let nfa₁ := loop r₁ nfa₂.val.start nfa₂
-
-  have property : nfa ≤ nfa₁ :=
-    calc nfa
-      _ ≤ nfa₂.val := nfa₂.property
-      _ ≤ nfa₁.val := nfa₁.property
-
-  have : result = ⟨nfa₁, property⟩ := by
-    simp [eq.symm, compile.loop]
-  exact motive nfa₂ nfa₁ property rfl rfl this
-
-theorem compile.loop.star (eq : compile.loop (Regex.star r) next nfa = result)
-  {motive : ∀nfa' start nfa'' nodes''' nfa''' isLt isLt' property',
-    nfa' = nfa.addNode .fail →
-    start = nfa'.val.start →
-    nfa'' = compile.loop r start nfa' →
-    nodes''' = nfa''.val.nodes.set ⟨start.val, isLt⟩ (.split nfa''.val.start next) →
-    nfa''' = ⟨nodes''', ⟨start.val, isLt'⟩⟩ →
-    result = ⟨nfa''', property'⟩ →
-    P
-  } : P := by
-  let nfa' := nfa.addNode .fail
-  let start := nfa'.val.start
-  let nfa'' := loop r start nfa'
-
-  have property : nfa ≤ nfa'' :=
-    calc nfa
-      _ ≤ nfa'.val := nfa'.property
-      _ ≤ nfa''.val := nfa''.property
-  have isLt : start.val < nfa''.val.nodes.size :=
-    Nat.lt_of_lt_of_le nfa'.val.start.isLt (NFA.le_size_of_le nfa''.property)
-
-  -- Patch the placeholder node
-  let nodes''' := nfa''.val.nodes.set ⟨start.val, isLt⟩ (.split nfa''.val.start next)
-
-  have eq_size : nodes'''.size = nfa''.val.nodes.size := by simp
-  have isLt' : start.val < nodes'''.size := eq_size ▸ isLt
-  let nfa''' : NFA := ⟨nodes''', ⟨start.val, isLt'⟩⟩
-
-  have property' : nfa ≤ nfa''' := by
-    intro i h
-
-    have le_size : nfa.nodes.size ≤ nfa''.val.nodes.size := NFA.le_size_of_le property
-    have h₂ : i < nodes'''.size := Nat.lt_of_lt_of_le h (eq_size ▸ le_size)
-    exists h₂
-
-    have eq : nfa'''[i] = nfa''.val[i]'(Nat.lt_of_lt_of_le h le_size) := by
-      apply Array.get_set_ne
-      exact (Nat.ne_of_gt h)
-    rw [eq]
-    exact (property i _).2
-
-  have : result = ⟨nfa''', property'⟩ := by
-    simp [eq.symm, compile.loop]
-  exact motive nfa' start nfa'' nodes''' nfa''' isLt isLt' property' rfl rfl rfl rfl rfl this
-
-theorem compile.loop.get_lt (eq : compile.loop r next nfa = result)
-  (h : i < nfa.nodes.size) :
-  result.val[i]'(Nat.lt_of_lt_of_le h (NFA.le_size_of_le (eq ▸ compile.loop.le))) = nfa[i] := by
-  induction r generalizing next nfa with
-  | empty | epsilon | char =>
-    try apply compile.loop.empty eq
-    try apply compile.loop.epsilon eq
-    try apply compile.loop.char eq
-    intro eq
-    subst eq
-    apply NFA.get_lt_addNode h
-  | alternate r₁ r₂ ih₁ ih₂ =>
-    apply compile.loop.alternate eq
-    intro nfa₁ start₁ nfa₂ start₂ nfa' property eq₁ _ eq₃ _ eq₅ eq
-
-    have h' : i < nfa₁.val.nodes.size :=
-      Nat.lt_of_lt_of_le h (NFA.le_size_of_le nfa₁.property)
-    have h'' : i < nfa₂.val.nodes.size :=
-      Nat.lt_of_lt_of_le h' (NFA.le_size_of_le nfa₂.property)
-
-    simp [eq, eq₅, NFA.get_lt_addNode h'']
-    simp [ih₂ eq₃.symm h']
-    simp [ih₁ eq₁.symm h]
-  | concat r₁ r₂ ih₁ ih₂ =>
-    apply compile.loop.concat eq
-    intro nfa₂ nfa₁ property eq₂ eq₁ eq
-
-    have h' : i < nfa₂.val.nodes.size :=
-      Nat.lt_of_lt_of_le h (NFA.le_size_of_le nfa₂.property)
-
-    simp [eq]
-    simp [ih₁ eq₁.symm h']
-    simp [ih₂ eq₂.symm h]
-  | star r ih =>
-    apply compile.loop.star eq
-    intro nfa' start nfa'' nodes''' nfa''' isLt isLt' property'
-      eq₁ eq₂ eq₃ eq₄ eq₅ eq
-
-    have h' : i < nfa'.val.nodes.size :=
-      Nat.lt_of_lt_of_le h (NFA.le_size_of_le nfa'.property)
-    have h'' : i < nfa''.val.nodes.size :=
-      Nat.lt_of_lt_of_le h' (NFA.le_size_of_le nfa''.property)
-    have ih := ih eq₃.symm h'
-    have ne : (Fin.mk start isLt).val ≠ i := by
-      simp [eq₂]
-      rw [eq₁]
-      simp [NFA.addNode]
-      exact Nat.ne_of_gt h
-
-    conv =>
-      lhs
-      simp [eq, eq₅, NFA.eq_get, eq₄]
-      rw [Array.get_set_ne nfa''.val.nodes ⟨start, isLt⟩ _ h'' ne]
-      simp [NFA.eq_get.symm, ih]
-      simp [eq₁, NFA.get_lt_addNode h]
-
--- The compiled NFA contains `.done` only at the first position
-theorem compile.loop.get_done_of_zero (eq : compile.loop r next nfa = result)
-  (assm : ∀i, (_ : i < nfa.nodes.size) → nfa[i] = .done → i = 0) :
-  ∀i, (_ : i < result.val.nodes.size) → result.val[i] = .done → i = 0 := by
-  induction r generalizing next nfa with
-  | empty | epsilon | char =>
-    try apply compile.loop.empty eq
-    try apply compile.loop.epsilon eq
-    try apply compile.loop.char eq
-
-    intro eq i h done
-    subst eq
-    cases Nat.lt_or_ge i nfa.nodes.size with
-    | inl lt =>
-      rw [NFA.get_lt_addNode lt] at done
-      exact assm i lt done
-    | inr ge =>
-      simp [NFA.addNode] at h
-      have : i = nfa.nodes.size := Nat.eq_of_ge_of_lt ge h
-      simp [this] at done
-  | alternate r₁ r₂ ih₁ ih₂ =>
-    apply compile.loop.alternate eq
-    intro nfa₁ start₁ nfa₂ start₂ nfa' property eq₁ _ eq₃ _ eq₅ eq i h done
-
-    have ih : i < nfa₂.val.nodes.size → i = 0 := by
-      intro h'
-      have done' : nfa₂.val[i] = .done := by
-        simp [eq, eq₅, NFA.get_lt_addNode h'] at done
-        exact done
-      apply ih₂ eq₃.symm _ i h' done'
-      exact ih₁ eq₁.symm assm
-
-    cases Nat.lt_or_ge i nfa₂.val.nodes.size with
-    | inl lt => exact ih lt
-    | inr ge =>
-      simp [eq, eq₅, NFA.addNode] at h
-      have : i = nfa₂.val.nodes.size := Nat.eq_of_ge_of_lt ge h
-      simp [this, eq, eq₅] at done
-  | concat r₁ r₂ ih₁ ih₂ =>
-    apply compile.loop.concat eq
-    intro nfa₂ nfa₁ property eq₂ eq₁ eq
-    simp [eq]
-    apply ih₁ eq₁.symm
-    apply ih₂ eq₂.symm assm
-  | star r ih =>
-    apply compile.loop.star eq
-    intro nfa' start nfa'' nodes''' nfa''' isLt isLt' property'
-      eq₁ _ eq₃ eq₄ eq₅ eq i h done
-
-    have assm' : ∀i, (_ : i < nfa'.val.nodes.size) → nfa'.val[i] = .done → i = 0 := by
-      intro i h done
-      cases Nat.lt_or_ge i nfa.nodes.size with
-      | inl lt =>
-        simp [eq₁, NFA.get_lt_addNode lt] at done
-        exact assm i lt done
-      | inr ge =>
-        simp [eq₁, NFA.addNode] at h
-        have : i = nfa.nodes.size := Nat.eq_of_ge_of_lt ge h
-        simp [this, eq₁] at done
-    have h' : i < nfa''.val.nodes.size := by
-      simp [eq, eq₅, eq₄] at h
-      exact h
-    have ih := ih eq₃.symm assm' i h'
-
-    simp [eq, eq₅, NFA.eq_get, eq₄, Array.get_set, h'] at done
-    split at done
-    . exact done.elim
-    . exact ih done
-
-theorem compile.get_done_iff_zero (eq : compile r = result) (h : i < result.nodes.size) :
-  result[i] = .done ↔ i = 0 := by
-  let init : NFA := compile.init
-  generalize eq' : compile.loop r 0 init = result'
-  have : result = result'.val := by
-    simp [eq.symm, compile, eq'.symm]
-  simp [this] at h
-  simp [this]
-
-  apply Iff.intro
-  . intro done
-    have assm : ∀i, (_ : i < init.nodes.size) → init[i] = .done → i = 0 := by
-      intro i h _
-      simp at h
-      match i with
-      | 0 => rfl
-      | i + 1 => contradiction
-    exact compile.loop.get_done_of_zero eq' assm i h done
-  . intro h
-    have h' : 0 < init.nodes.size := by decide
-    simp [h, eq'.symm]
-    apply compile.loop.get_lt rfl h'
-
-theorem compile.loop.inBounds (eq : compile.loop r next nfa = result)
-  (h₁ : next < nfa.nodes.size) (h₂ : nfa.inBounds) :
-  result.val.inBounds := by
-  induction r generalizing next nfa with
-  | empty | epsilon | char =>
-    try apply compile.loop.empty eq
-    try apply compile.loop.epsilon eq
-    try apply compile.loop.char eq
-
-    intro eq i
-    subst eq
-    have h' : next < nfa.nodes.size + 1 := lt_trans h₁ (Nat.lt_succ_self _)
-
-    cases Nat.lt_or_ge i nfa.nodes.size with
-    | inl lt =>
-      simp [NFA.get_lt_addNode lt]
-      exact Node.inBounds_of_inBounds_of_le (h₂ ⟨i, lt⟩) (by simp [NFA.addNode]; exact Nat.le_succ _)
-    | inr ge =>
-      let lt := i.isLt
-      simp only [NFA.addNode, Array.size_push] at lt
-      have : i = nfa.nodes.size := Nat.eq_of_ge_of_lt ge lt
-      simp [this]
-      try simp [NFA.addNode]
-      try exact Node.inBounds.epsilon h'
-      try exact Node.inBounds.char h'
-  | alternate r₁ r₂ ih₁ ih₂ =>
-    apply compile.loop.alternate eq
-    intro nfa₁ start₁ nfa₂ start₂ nfa' property eq₁ _ eq₃ _ eq₅ eq i
-
-    have ih : i < nfa₂.val.nodes.size → result.val[i].inBounds result.val.nodes.size := by
-      intro h
-      simp [eq, eq₅]
-      simp [NFA.get_lt_addNode h]
-      simp [NFA.addNode]
-      have ih₁ := ih₁ eq₁.symm h₁ h₂
-      have ih₂ := ih₂ eq₃.symm (Nat.lt_of_lt_of_le h₁ (NFA.le_size_of_le nfa₁.property)) ih₁
-      exact Node.inBounds_of_inBounds_of_le (ih₂ ⟨i, h⟩) (Nat.le_succ _)
-
-    cases Nat.lt_or_ge i nfa₂.val.nodes.size with
-    | inl lt => exact ih lt
-    | inr ge =>
-      let lt := i.isLt
-      simp only [eq, eq₅, NFA.addNode, Array.size_push] at lt
-      have : i = nfa₂.val.nodes.size := Nat.eq_of_ge_of_lt ge lt
-      simp [eq, eq₅, this]
-      simp [NFA.addNode]
-      apply Node.inBounds.split
-      . exact lt_trans start₁.isLt (Nat.lt_of_le_of_lt (NFA.le_size_of_le nfa₂.property) (Nat.lt_succ_self _))
-      . exact lt_trans start₂.isLt (Nat.lt_succ_self _)
-  | concat r₁ r₂ ih₁ ih₂ =>
-    apply compile.loop.concat eq
-    intro nfa₂ nfa₁ property eq₂ eq₁ eq
-    simp [eq]
-    apply ih₁ eq₁.symm nfa₂.val.start.isLt
-    apply ih₂ eq₂.symm h₁ h₂
-  | star r ih =>
-    apply compile.loop.star eq
-    intro nfa' start nfa'' nodes''' nfa''' isLt isLt' property'
-      eq₁ _ eq₃ eq₄ eq₅ eq i
-
-    have eqsize : result.val.nodes.size = nfa''.val.nodes.size := by
-      simp [eq, eq₅, eq₄]
-    have h' : i < nfa''.val.nodes.size :=
-      calc
-        i < result.val.nodes.size := i.isLt
-        _ = _ := eqsize
-    have inBounds' : nfa'.val.inBounds := by
-      simp [eq₁]
-      intro i
-      cases Nat.lt_or_ge i nfa.nodes.size with
-      | inl lt =>
-        simp [NFA.get_lt_addNode lt]
-        exact Node.inBounds_of_inBounds_of_le (h₂ ⟨i, lt⟩) (by simp [NFA.addNode]; exact Nat.le_succ _)
-      | inr ge =>
-        let lt := i.isLt
-        simp only [NFA.addNode, Array.size_push] at lt
-        have : i = nfa.nodes.size := Nat.eq_of_ge_of_lt ge lt
-        simp [this]
-    have ih := ih eq₃.symm start.isLt inBounds'
-
-    simp [eq, eq₅, NFA.eq_get, eq₄, Array.get_set, h']
-    split
-    . apply Node.inBounds.split
-      . exact nfa''.val.start.isLt
-      . exact Nat.lt_of_lt_of_le h₁ (NFA.le_size_of_le (le_trans nfa'.property nfa''.property))
-    . exact ih (i.cast eqsize)
-
-theorem compile.init.inBounds : compile.init.inBounds := by
-  intro i
-  simp [NFA.eq_get, init, Array.singleton_get']
-
-theorem compile.inBounds (eq : compile r = result) : result.inBounds := by
-  simp [eq.symm, compile]
-  exact compile.loop.inBounds rfl (by decide) compile.init.inBounds
-
-theorem compile.init.get : compile.init[0] = .done := by
-  simp [compile.init, NFA.eq_get, Array.singleton_get']
-
--- When we compile a new regex into an existing NFA, the compiled nodes first
--- "circulates" within the new nodes, then "escape" to the `next` node.
-
-def compile.loop.NewNodesRange (_ : compile.loop r next nfa = result) : Set Nat :=
-  { i | nfa.nodes.size ≤ i ∧ i < result.val.nodes.size }
-
-theorem compile.loop.start_in_NewNodesRange (eq : compile.loop r next nfa = result) :
-  result.val.start.val ∈ NewNodesRange eq := by
-  simp [NewNodesRange]
-  induction r generalizing next nfa with
-  | empty =>
-    apply compile.loop.empty eq
-    intro eq
-    rw [eq]
-    simp [NFA.addNode]
-  | epsilon =>
-    apply compile.loop.epsilon eq
-    intro eq
-    rw [eq]
-    simp [NFA.addNode]
-  | char c =>
-    apply compile.loop.char eq
-    intro eq
-    rw [eq]
-    simp [NFA.addNode]
-  | alternate r₁ r₂ =>
-    apply compile.loop.alternate eq
-    intro nfa₁ start₁ nfa₂ start₂ nfa' property _ _ _ _ eq₅ eq
-    rw [eq]
-    simp
-    rw [eq₅]
-    simp [NFA.addNode]
-    exact NFA.le_size_of_le (le_trans nfa₁.property nfa₂.property)
-  | concat r₁ r₂ ih₁ =>
-    apply compile.loop.concat eq
-    intro nfa₂ nfa₁ property _ eq₁ eq
-    rw [eq]
-    simp
-    have ih₁ := ih₁ eq₁.symm
-    exact le_trans (NFA.le_size_of_le nfa₂.property) ih₁
-  | star r =>
-    apply compile.loop.star eq
-    intro nfa' start nfa'' nodes''' nfa''' isLt isLt' property'
-      eq₁ eq₂ _ _ eq₅ eq
-    rw [eq]
-    simp
-    rw [eq₅]
-    simp [eq₂]
-    rw [eq₁]
-    simp [NFA.addNode]
-
-theorem compile.start_gt (eq : compile r = nfa) : 0 < nfa.start.val := by
-  generalize eq' : compile.loop r 0 compile.init = result
-  have : nfa = result.val := by
-    simp [eq.symm, compile, eq'.symm]
-  rw [this]
-  have inRange := compile.loop.start_in_NewNodesRange eq'
-  simp [compile.loop.NewNodesRange, compile.init] at inRange
-  exact inRange
-
-theorem compile.loop.step_range (eq : compile.loop r next nfa = result) :
-  ∀ i, nfa.nodes.size ≤ i → (_ : i < result.val.nodes.size) →
-  (∀ c, result.val[i].charStep c ⊆ {next} ∪ NewNodesRange eq) ∧
-  result.val[i].εStep ⊆ {next} ∪ NewNodesRange eq := by
-  induction r generalizing next nfa with
-  | empty =>
-    apply compile.loop.empty eq
-    intro eq i h₁ h₂
-    simp [eq, NFA.addNode] at h₂
-    have h : i = nfa.nodes.size := Nat.eq_of_ge_of_lt h₁ h₂
-    simp [eq, h, Node.charStep, Node.εStep]
-  | epsilon =>
-    apply compile.loop.epsilon eq
-    intro eq i h₁ h₂
-    simp [eq, NFA.addNode] at h₂
-    have h : i = nfa.nodes.size := Nat.eq_of_ge_of_lt h₁ h₂
-    simp [eq, h, Node.charStep, Node.εStep]
-  | char c' =>
-    apply compile.loop.char eq
-    intro eq i h₁ h₂
-    simp [eq, NFA.addNode] at h₂
-    have h : i = nfa.nodes.size := Nat.eq_of_ge_of_lt h₁ h₂
-    simp [eq, h, Node.charStep, Node.εStep]
-    intro c
-    apply le_trans
-    . show (if c = c' then {next} else ∅) ≤ {next}
-      simp
-    . simp
-  | alternate r₁ r₂ ih₁ ih₂ =>
-    apply compile.loop.alternate eq
-    intro nfa₁ start₁ nfa₂ start₂ nfa' property eq₁ eq₂ eq₃ eq₄ eq₅ eq i h₁ h₂
-    simp [NewNodesRange, eq]
-
-    have size : i < nfa'.val.nodes.size := by
-      simp [eq] at h₂
-      exact h₂
-    have size₂ : nfa₂.val.nodes.size < nfa'.val.nodes.size := by
-      simp [eq₅]
-      exact NFA.lt_size_addNode
-    have size₁ : nfa₁.val.nodes.size < nfa'.val.nodes.size :=
-      Nat.lt_of_le_of_lt (NFA.le_size_of_le nfa₂.property) size₂
-
-    cases Nat.lt_or_ge i nfa₁.val.nodes.size with
-    | inl lt =>
-      have ih₁ := ih₁ eq₁.symm i h₁ lt
-      have : nfa'.val[i] = nfa₁.val[i] := by
-        simp [eq₅]
-        rw [NFA.get_lt_addNode (Nat.lt_of_lt_of_le lt (NFA.le_size_of_le nfa₂.property))]
-        rw [get_lt eq₃.symm lt]
-      rw [this]
-      have : {next} ∪ NewNodesRange eq₁.symm ⊆
-        {next} ∪ {i | nfa.nodes.size ≤ i ∧ i < nfa'.val.nodes.size} := by
-        apply Set.insert_subset_insert
-        apply Set.setOf_subset_setOf.mpr
-        intro i h
-        exact ⟨h.left, lt_trans h.right size₁⟩
-      exact ⟨fun c => le_trans (ih₁.left c) this, le_trans ih₁.right this⟩
-    | inr ge =>
-      cases Nat.lt_or_ge i nfa₂.val.nodes.size with
-      | inl lt =>
-        have ih₂ := ih₂ eq₃.symm i ge lt
-        have : nfa'.val[i] = nfa₂.val[i] := by
-          simp [eq₅]
-          rw [NFA.get_lt_addNode lt]
-        rw [this]
-        have : {next} ∪ NewNodesRange eq₃.symm ⊆
-          {next} ∪ {i | nfa.nodes.size ≤ i ∧ i < nfa'.val.nodes.size} := by
-          apply Set.insert_subset_insert
-          apply Set.setOf_subset_setOf.mpr
-          intro i h
-          exact ⟨le_trans (NFA.le_size_of_le nfa₁.property) h.left, lt_trans h.right size₂⟩
-        exact ⟨fun c => le_trans (ih₂.left c) this, le_trans ih₂.right this⟩
-      | inr ge =>
-        simp [eq, eq₅, NFA.addNode] at h₂
-        have h : i = nfa₂.val.nodes.size := Nat.eq_of_ge_of_lt ge h₂
-        have : nfa'.val[i] = (.split nfa₁.val.start nfa₂.val.start) := by
-          simp [eq₅, h, eq₂, eq₄]
-        simp [this, Node.charStep, Node.εStep]
-        apply Set.insert_subset
-        . simp
-          have h := start_in_NewNodesRange eq₁.symm
-          exact .inr ⟨h.left, lt_trans h.right size₁⟩
-        . simp
-          have h := start_in_NewNodesRange eq₃.symm
-          exact .inr ⟨le_trans (NFA.le_size_of_le nfa₁.property) h.left, lt_trans h.right size₂⟩
-  | concat r₁ r₂ ih₁ ih₂ =>
-    apply compile.loop.concat eq
-    intro nfa₂ nfa₁ property eq₂ eq₁ eq i h₁ h₂
-    simp [NewNodesRange, eq]
-
-    have size : i < nfa₁.val.nodes.size := by
-      simp [eq] at h₂
-      exact h₂
-    have size' : nfa₂.val.nodes.size ≤ nfa₁.val.nodes.size :=
-      NFA.le_size_of_le nfa₁.property
-
-    cases Nat.lt_or_ge i nfa₂.val.nodes.size with
-    | inl lt =>
-      have ih₂ := ih₂ eq₂.symm i h₁ lt
-      have : nfa₁.val[i] = nfa₂.val[i] := get_lt eq₁.symm lt
-      rw [this]
-      have : {next} ∪ NewNodesRange eq₂.symm ⊆
-        {next} ∪ {i | nfa.nodes.size ≤ i ∧ i < nfa₁.val.nodes.size} := by
-        apply Set.insert_subset_insert
-        apply Set.setOf_subset_setOf.mpr
-        intro i h
-        exact ⟨h.left, Nat.lt_of_lt_of_le h.right size'⟩
-      exact ⟨fun c => le_trans (ih₂.left c) this, le_trans ih₂.right this⟩
-    | inr ge =>
-      have ih₁ := ih₁ eq₁.symm i ge size
-      have : {nfa₂.val.start.val} ∪ NewNodesRange eq₁.symm ⊆
-        {next} ∪ {i | nfa.nodes.size ≤ i ∧ i < nfa₁.val.nodes.size} := by
-        apply Set.union_subset
-        . simp
-          have h := start_in_NewNodesRange eq₂.symm
-          exact .inr ⟨h.left, Nat.lt_of_lt_of_le h.right size'⟩
-        . simp [Set.subset_def]
-          intro i h
-          exact .inr ⟨le_trans (NFA.le_size_of_le nfa₂.property) h.left, h.right⟩
-      exact ⟨fun c => le_trans (ih₁.left c) this, le_trans ih₁.right this⟩
-  | star r ih =>
-    apply compile.loop.star eq
-    intro nfa' start nfa'' nodes''' nfa''' isLt isLt' property'
-      eq₁ eq₂ eq₃ eq₄ eq₅ eq i h₁ h₂
-    simp [NewNodesRange, eq]
-
-    have eqs : start.val = nfa.nodes.size := by
-      simp [eq₂]
-      rw [eq₁]
-      simp [NFA.addNode]
-    have size : i < nfa'''.nodes.size := by
-      simp [eq] at h₂
-      exact h₂
-    have eqsize : nfa''.val.nodes.size = nfa'''.nodes.size := by
-      simp [eq₅, eq₄]
-    have size'' : i < nfa''.val.nodes.size := eqsize ▸ size
-
-    cases Nat.lt_or_ge i nfa'.val.nodes.size with
-    | inl lt =>
-      simp [eq₁, NFA.addNode] at lt
-      have h := Nat.eq_of_ge_of_lt h₁ lt
-      have : nfa'''[i] = .split nfa''.val.start next := by
-        have : i = start := by
-          rw [h, eqs]
-        simp [this, eq₅, NFA.eq_get, eq₄]
-      simp [this, Node.charStep, Node.εStep]
-      apply Set.insert_subset
-      . have h := start_in_NewNodesRange eq₃.symm
-        simp
-        exact .inr ⟨le_trans (NFA.le_size_of_le nfa'.property) h.left, eqsize ▸ nfa''.val.start.isLt⟩
-      . simp
-    | inr ge =>
-      have ih := ih eq₃.symm i ge size''
-      have : nfa'''[i] = nfa''.val[i] := by
-        simp [eq₅, NFA.eq_get, eq₄]
-        apply Array.get_set_ne
-        rw [eqs]
-        apply Nat.ne_of_lt
-        have : nfa.nodes.size + 1 ≤ i := by
-          simp [eq₁, NFA.addNode] at ge
-          exact ge
-        exact this
-      rw [this]
-      have : {start.val} ∪ NewNodesRange eq₃.symm ⊆
-        {next} ∪ {i | nfa.nodes.size ≤ i ∧ i < nfa'''.nodes.size} := by
-        apply Set.union_subset
-        . simp
-          have : start.val < nfa'''.nodes.size :=
-            calc start.val
-              _ < nfa'.val.nodes.size := start.isLt
-              _ ≤ nfa''.val.nodes.size := NFA.le_size_of_le nfa''.property
-              _ = nfa'''.nodes.size := eqsize
-          exact .inr ⟨eqs ▸ le_refl _, this⟩
-        . simp [Set.subset_def]
-          intro i h
-          exact .inr ⟨le_trans (NFA.le_size_of_le nfa'.property) h.left, eqsize ▸ h.right⟩
-      exact ⟨fun c => le_trans (ih.left c) this, le_trans ih.right this⟩
-
-theorem compile.loop.lt_size (eq : compile.loop r next nfa = result) :
-  nfa.nodes.size < result.val.nodes.size := by
-  induction r generalizing next nfa with
-  | empty =>
-    apply compile.loop.empty eq
-    intro eq
-    simp [eq, NFA.addNode]
-  | epsilon =>
-    apply compile.loop.epsilon eq
-    intro eq
-    simp [eq, NFA.addNode]
-  | char c' =>
-    apply compile.loop.char eq
-    intro eq
-    simp [eq, NFA.addNode]
-  | alternate r₁ r₂ ih₁ ih₂ =>
-    apply compile.loop.alternate eq
-    intro nfa₁ start₁ nfa₂ start₂ nfa' property eq₁ _ eq₃ _ eq₅ eq
-    simp [eq, eq₅, NFA.addNode]
-    calc nfa.nodes.size
-      _ < nfa₁.val.nodes.size := ih₁ eq₁.symm
-      _ < nfa₂.val.nodes.size := ih₂ eq₃.symm
-      _ < _ := Nat.lt_succ_self _
-  | concat r₁ r₂ ih₁ ih₂ =>
-    apply compile.loop.concat eq
-    intro nfa₂ nfa₁ property eq₂ eq₁ eq
-    simp [eq]
-    calc nfa.nodes.size
-      _ < nfa₂.val.nodes.size := ih₂ eq₂.symm
-      _ < nfa₁.val.nodes.size := ih₁ eq₁.symm
-  | star r _ =>
-    apply compile.loop.star eq
-    intro placeholder loopStart compiled nodes patched isLt isLt' property'
-      eq₁ _ _ eq₄ eq₅ eq'
-    calc nfa.nodes.size
-      _ < placeholder.val.nodes.size := by simp [eq₁, NFA.addNode]
-      _ ≤ compiled.val.nodes.size := NFA.le_size_of_le compiled.property
-      _ = _ := by
-        rw [eq']
-        simp [eq₅, eq₄]
-
-theorem compile.loop.star.loopStartNode (eq : compile.loop (.star r) next nfa = result) :
-  ∃ rStart ∈ { i | nfa.nodes.size + 1 ≤ i ∧ i < result.val.nodes.size },
-  result.val[nfa.nodes.size]'(compile.loop.lt_size eq) = .split rStart next := by
-  apply compile.loop.star eq
-  intro placeholder loopStart compiled nodes patched isLt isLt' property'
-    eq₁ eq₂ eq₃ eq₄ eq₅ eq'
-  exists compiled.val.start.val
-  have : nfa.nodes.size = (Fin.mk loopStart.val isLt).val := by
-    simp [eq₂]
-    rw [eq₁]
-    simp [NFA.addNode]
-  simp [this, eq', eq₅, NFA.eq_get, eq₄]
-  calc loopStart.val + 1
-    _ ≤ placeholder.val.nodes.size := loopStart.isLt
-    _ ≤ _ := by
-      have startRange := compile.loop.start_in_NewNodesRange eq₃.symm
-      simp [NewNodesRange] at startRange
-      exact startRange
-
-@[simp]
-theorem compile.loop.star.charStep_loopStartNode {c} (eq : compile.loop (.star r) next nfa = result) :
-  (result.val[nfa.nodes.size]'(compile.loop.lt_size eq)).charStep c = ∅ := by
-  let ⟨_, _, eq⟩ := compile.loop.star.loopStartNode eq
-  simp [eq, Node.charStep]
 
 end NFA
