Regex.lean
@@ -1,4 +1,3 @@
 import Regex.Regex
-import Regex.Derivative
 import Regex.NFA
 import Regex.Parser
