Regex/NFA/VM.lean
@@ -1,2 +1,1 @@
 import Regex.NFA.VM.Basic
-import Regex.NFA.VM.Correctness
